% Equation 1
\begin{dmath}
{\bar{Y}_{t}}={\bar{Y}_{t-1}}+{\epsilon^{\bar{Y}}_{t}}
\end{dmath}
% Equation 2
\begin{dmath}
{R^{US}_{t}}={\kappa}\, \left({R^{US}_{t-1}}-{\bar{R}^{US}_{t-1}}\right)+{\epsilon^{R^{US}}_{t}}+{\bar{R}^{US}_{t}}
\end{dmath}
% Equation 3
\begin{dmath}
{R_{t}}={I_{t}}-{\pi_{t+12}}
\end{dmath}
% Equation 4
\begin{dmath}
{\bar{Z}_{t}}={\bar{Z}_{t-1}}+{\epsilon^{\bar{Z}}_{t}}
\end{dmath}
% Equation 5
\begin{dmath}
{Z_{t+1}}={Z_{t+1}}\, {\phi}+\left(1-{\phi}\right)\, {Z_{t-1}}
\end{dmath}
% Equation 6
\begin{dmath}
{y_{t}}={Y_{t}}-{\bar{Y}_{t}}
\end{dmath}
% Equation 7
\begin{dmath}
{y_{t}}={\beta_{1}}\, {y_{t-1}}-{\beta_{2}}\, {y_{t+1}}-{\beta_{3}}\, {R_{t-1}}+{Z_{t-1}}\, {\beta_{4}}+{\chi_{t}}
\end{dmath}
% Equation 8
\begin{dmath}
{r_{t}}={R_{t}}-{\bar{R}_{t}}
\end{dmath}
% Equation 9
\begin{dmath}
{z_{t}}={Z_{t}}-{\bar{Z}_{t}}
\end{dmath}
% Equation 10
\begin{dmath}
{\chi_{t}}={\rho_{y}}\, {\chi_{t-1}}+{\epsilon^{Y}_{t}}
\end{dmath}
% Equation 11
\begin{dmath}
{\Psi_{t}}={\rho_{y}}\, {\Psi_{t-1}}+{\epsilon^{\pi}_{t}}
\end{dmath}
% Equation 12
\begin{dmath}
{\pi_{t}}={\Psi_{t}}+{\pi_{t+12}}\, {\lambda_{1}}+\left(1-{\lambda_{1}}\right)\, {\pi_{t-1}}+{\lambda_{2}}\, {Y_{t-1}}+{\lambda_{3}}\, \left({Z_{t}}-{Z_{t-12}}\right)
\end{dmath}
% Equation 13
\begin{dmath}
{I_{t}}={\gamma_{1}}\, {I_{t-1}}+\left(1-{\gamma_{1}}\right)\, \left({\pi_{t+12}}+{\bar{R}_{t}}+{\gamma_{2}}\, \left({\pi_{t+12}}-{\pi^{TAR}_{t}}\right)+{y_{t}}\, {\gamma_{3}}\right)+{\epsilon^{I}_{t}}
\end{dmath}
% Equation 14
\begin{dmath}
12\, \left({Z_{t+1}}-{Z_{t-1}}\right)={R_{t}}-{R^{US}_{t}}-\left({\bar{R}_{t}}-{\bar{R}^{US}_{t}}\right)+{\epsilon^{Z-Z^{e}}_{t}}
\end{dmath}
% Equation 15
\begin{dmath}
{\bar{R}_{t}}={\rho}\, {r_{ss}}+\left(1-{\rho}\right)\, {\bar{R}_{t-1}}+{\epsilon^{\bar{R}}_{t}}
\end{dmath}
% Equation 16
\begin{dmath}
{\bar{R}^{US}_{t}}=\left(1-{\rho_{US}}\right)\, {r^{US}_{ss}}+{\bar{R}^{US}_{t-1}}\, {\rho_{US}}+{\epsilon^{\bar{R^{US}}}_{t}}
\end{dmath}
